Cslib/Computability/Machines/MultiTapeTuring/SequentialCombinator.lean
@@ -16,40 +16,40 @@ namespace Turing
 
 namespace MultiTapeTM
 
-variable [Inhabited α]
+variable [Inhabited Symbol] [Fintype Symbol]
 variable {k : ℕ}
 
 /--
 Sequential combination of Turing machines. Runs `tm₁` and then `tm₂` on the resulting tapes
 (if the first one halts).
 -/
-public def seq (tm₁ tm₂ : MultiTapeTM k α) : MultiTapeTM k α := sorry
+public def seq (tm₁ tm₂ : MultiTapeTM k Symbol) : MultiTapeTM k Symbol := sorry
 
 public theorem seq_eval
-  (tm₁ tm₂ : MultiTapeTM k α)
-  (tapes₀ : Fin k → BiTape α) :
+  (tm₁ tm₂ : MultiTapeTM k Symbol)
+  (tapes₀ : Fin k → BiTape Symbol) :
   (seq tm₁ tm₂).eval tapes₀ =
     tm₁.eval tapes₀ >>= fun tape₁ => tm₂.eval tape₁ := by
   sorry
 
 @[simp, grind =]
 public theorem seq_eval_list
-  {tm₁ tm₂ : MultiTapeTM k (WithSep α)}
-  {tapes₀ : Fin k → List (List α)} :
+  {tm₁ tm₂ : MultiTapeTM k (WithSep Symbol)}
+  {tapes₀ : Fin k → List (List Symbol)} :
   (seq tm₁ tm₂).eval_list tapes₀ =
     tm₁.eval_list tapes₀ >>= fun tape₁ => tm₂.eval_list tape₁ := by
   sorry
 
 public theorem seq_associative
-  (tm₁ tm₂ tm₃ : MultiTapeTM k α)
-  (tapes₀ : Fin k → List (List α)) :
+  (tm₁ tm₂ tm₃ : MultiTapeTM k Symbol)
+  (tapes₀ : Fin k → List (List Symbol)) :
   (seq (seq tm₁ tm₂) tm₃).eval = (seq tm₁ (seq tm₂ tm₃)).eval := by
   sorry
 
 /--
 Sequential combination of Turing machines.
 -/
-infixl:90 " <;> " => seq
+infixl:90 " ;ₜ " => seq
 
 
 end MultiTapeTM
