Cslib/Computability/Machines/MultiTapeTuring/WhileCombinator.lean
@@ -26,9 +26,10 @@ at the head of tape `i` is true.
 -/
 public def doWhileSymbol (cond : Option α → Bool) (i : Fin k) (tm : MultiTapeTM k α) :
     MultiTapeTM k α where
-  Λ := PUnit
-  q₀ := 0
-  M _ syms := sorry
+  State := PUnit
+  stateFintype := inferInstance
+  q₀ := PUnit.unit
+  tr _ syms := sorry
 
 @[simp]
 public theorem doWhileSymbol_eval
@@ -45,16 +46,17 @@ public theorem doWhileSymbol_eval
 -/
 public def doWhile (i : Fin k) (tm : MultiTapeTM k (WithSep α)) :
     MultiTapeTM k (WithSep α) where
-  Λ := PUnit
-  q₀ := 0
-  M _ syms := sorry
+  State := PUnit
+  stateFintype := inferInstance
+  q₀ := PUnit.unit
+  tr _ syms := sorry
 
 @[simp]
 public theorem doWhile_eval_list
   {i : Fin k}
   {tm : MultiTapeTM k (WithSep α)}
   {tapes : Fin k → List (List α)}
-  (h_halts : ∀ tapes', tm.HaltsOnLists tapes') :
+  (h_halts : ∀ tapes', (tm.eval_list tapes').Dom) :
   (doWhile i tm).eval_list tapes =
     ⟨∃ n, ((tm.eval_list_tot h_halts)^[n] tapes i).head?.getD [] = [],
       fun h_loopEnds => (tm.eval_list_tot h_halts)^[Nat.find h_loopEnds] tapes⟩ := by
